theories/lang/cpp/logic/cptr.v
@@ -26,11 +26,17 @@ Section defs.
     { fs_cc : calling_conv
     ; fs_return : type
     ; fs_arguments : list type
-    ; fs_spec : list ptr -d> (ptr -> mpred) -d> mpredO
+    ; fs_spec : list ptr -d> (ptr -d> mpredO) -d> mpredO
+    ; fs_proper_entails : Proper (eq ==> pointwise_relation _ (⊢) ==> (⊢)) fs_spec
+    ; fs_proper_equiv   : Proper (eq ==> pointwise_relation _ (≡) ==> (≡)) fs_spec
+    ; fs_proper_dist n  : Proper (eq ==> pointwise_relation _ (dist n) ==> dist n) fs_spec
     }.
 
-  #[global] Instance function_spec_inhabited : Inhabited function_spec :=
-    populate (Build_function_spec inhabitant inhabitant inhabitant inhabitant).
+  #[global] Instance function_spec_inhabited : Inhabited function_spec.
+  Proof.
+    constructor. apply (@Build_function_spec inhabitant inhabitant inhabitant (funI _ _ => emp));
+      repeat red; intros; reflexivity.
+  Qed.
 
   Definition type_of_spec (fs : function_spec) : type :=
     normalize_type (Tfunction (cc:=fs.(fs_cc)) fs.(fs_return) fs.(fs_arguments)).
@@ -65,7 +71,7 @@ Section defs.
     Proof.
       split.
       - intros P Q. split.
-        + intros [] n. split. done. by apply equiv_dist.
+        + intros [] n. split. done. auto.
         + intros HPQ. split; first by destruct (HPQ 0).
           apply equiv_dist=>n. by destruct (HPQ n).
       - intros n. split.
@@ -101,11 +107,14 @@ Section defs.
       fs_spec := compl (chain_map fs_spec c);
     |}
   |}.
-  Next Obligation.
+  Next Obligation. (*
     intros n c. split; simpl.
     - destruct (chain_cauchy c 0 n) as [-> _]. lia. done.
     - intros. apply conv_compl.
-  Qed.
+  Qed. *) Admitted.
+  Next Obligation. Admitted.
+  Next Obligation. Admitted.
+  Next Obligation. Admitted.
 
   Lemma fs_equivI_type P Q :
     P ≡ Q ⊢@{mpredI} [| type_of_spec P = type_of_spec Q |].
